Abstracted from ident type

template-coq/theories/utils/MCEquality.v
@@ -1,4 +1,6 @@
 
+Require Bool.
+
 Definition transport {A} (P : A -> Type) {x y : A} (e : x = y) : P x -> P y
   := fun u => eq_rect x P u y e.
 
@@ -8,3 +10,38 @@ Notation "p # x" := (transport _ p x) (right associativity, at level 65).
 Lemma eq_rect_transport A x P u y p
   : @eq_rect A x P u y p = transport P p u.
 Proof. reflexivity. Defined.
+
+Definition eqdec A := forall (x y : A), {x = y} + {x <> y}.
+
+Definition booldec_spec {A} (f : A -> A -> bool) := 
+  forall x y, f x y = true <-> x = y.
+
+Definition eqdec_bdec {A} (E : eqdec A) : {f | @booldec_spec A f}.
+Proof.
+  exists (fun x y => if E x y then true else false).
+  intros x y. destruct (E x y); firstorder congruence.
+Defined.
+
+Definition bdec_eqdec {A} f (H : @booldec_spec A f) : eqdec A.
+Proof.
+  intros x y. destruct (f x y) eqn:E.
+  - left. now apply H.
+  - right. intros H2. destruct (H x y) as [_ H3]. specialize (H3 H2). congruence.
+Defined.
+
+Definition booldec_refl {A} f := forall (x y : A), Bool.reflect (x = y) (f x y).
+
+Lemma bdec_refl_spec {A} f :
+    @booldec_refl A f -> booldec_spec f.
+Proof.
+  intros H x y. specialize (H x y). enough (x = y <-> f x y = true) by tauto.
+  now eapply Bool.reflect_iff. 
+Qed.
+
+Lemma bdec_spec_relf {A} f :
+    @booldec_spec A f -> booldec_refl f.
+Proof.
+  intros H x y. specialize (H x y). assert (x = y <-> f x y = true) by tauto.
+  now eapply Bool.iff_reflect.
+Qed.
+
