template-coq/theories/AstUtils.v
@@ -1,5 +1,5 @@
 From Coq Require Import Ascii String Bool OrderedType Lia Arith.
-From MetaCoq.Template Require Import BasicAst Ast utils.
+From MetaCoq.Template Require Import Ast utils.
 Import List.ListNotations.
 Require Import ssreflect.
 Local Open Scope string_scope.
@@ -94,7 +94,7 @@ Fixpoint lookup_mind_decl (id : kername) (decls : global_env)
 
 Definition universes_entry_of_decl (u : universes_decl) : universes_entry :=
   match u with
-  | Polymorphic_ctx ctx => Polymorphic_entry (fst ctx) (Universes.AUContext.repr ctx)
+  | Polymorphic_ctx ctx => Polymorphic_entry (fst ctx) (AUContext.repr ctx)
   | Monomorphic_ctx ctx => Monomorphic_entry ctx
   end.
 
