template-coq/theories/Ident.v
@@ -1,0 +1,50 @@
+
+From Coq Require Import String.
+From MetaCoq.Template Require Import utils.
+
+Definition lt {s} cmp (a b : s) := cmp a b = Lt.
+
+Module Type Sig.
+    Parameter t : Set.
+
+    Parameter print : t -> string.
+
+    Parameter eqdec : eqdec t.
+    Parameter eq : t -> t -> bool.
+    Parameter eq_spec : booldec_spec eq.
+
+    Parameter cmp : t -> t -> comparison.
+    Parameter cmp_eq : forall x y, cmp x y = Eq <-> x = y.
+
+    Parameter lt_irreflexive : forall a, ~ (lt cmp a a).
+    Parameter lt_trans : forall a b c, lt cmp a b -> lt cmp b c -> lt cmp a c.
+End Sig.
+
+
+Module Native <: Sig.
+    Definition t := nstring.
+    Definition print := nstring_to_string.
+    Definition eqdec := nstring_eqdec.
+    Definition eq := nstring_eqb.
+    Definition eq_spec := nstring_eqb_correct.
+    Definition cmp := nstring_compare.
+    Definition cmp_eq := nstring_compare_eq.
+    Definition lt_irreflexive := nstring_lt_irreflexive.
+    Definition lt_trans := nstring_order_trans Lt.
+End Native.
+
+Module String <: Sig.
+    Definition t := string.
+    Definition print (x : string) := x.
+    Definition eqdec := String.string_dec.
+    Definition eq := String.eqb.
+    Definition eq_spec : booldec_spec eq.
+    Proof.
+        apply bdec_refl_spec. intros x y. apply String.eqb_spec.
+    Qed.
+
+    Definition cmp := string_compare.
+    Definition cmp_eq := string_compare_eq.
+    Definition lt_irreflexive := string_lt_irreflexive.
+    Definition lt_trans := transitive_string_lt.
+End String.
